proof/correctness/SignProof.ec
@@ -3,17 +3,17 @@ pragma Goals : printall.
 require import AllCore List RealExp IntDiv Distr DList IntDiv.
 from Jasmin require import JModel JArray.
 
-require import Types Params Parameters Address Notation Hash Primitives Wots XMSS_Commons XMSS_MT_PRF.
-require import XMSS_IMPL.
+require import Params Types Hash XMSS_MT_PRF.
+require import XMSS_IMPL Parameters.
 
-require import Repr. 
-require import Util Utils.
+require import Repr2. 
+require import Utils2.
 
 require import Array4 Array8 Array32 Array64 Array68 Array96 Array132 Array136 Array352 Array2144.
 require import WArray32 WArray96 WArray136.
 
 require import Correctness_Address Correctness_Mem Correctness_Hash.
-require import Utils DistrUtils.
+require import DistrUtils.
 
 require import BitEncoding.
 (*---*) import BitChunking.
@@ -33,39 +33,158 @@ arg{2}.`1 => sk
 arg{2}.`2 => msg
 *)
 
-print mkseq. 
-
 
 op load_message (mem : global_mem_t) (ptr : W64.t) (mlen : W64.t) =
   mkseq (fun (i : int) => mem.[to_uint ptr + i]) (to_uint mlen).
 
 
-lemma verify_correct (_sk : W8.t Array132.t, _sm_ptr _smlen_ptr _m_ptr _mlen : W64.t) :
+lemma sign_correct (mem : global_mem_t) (_sk : xmss_sk, _sm_ptr _smlen_ptr _m_ptr _mlen : W64.t) :
+    n = XMSS_N /\ 
+    prf_padding_val = XMSS_HASH_PADDING_PRF /\ 
+    padding_len = XMSS_PADDING_LEN =>
     equiv [
       M(Syscall).__xmssmt_core_sign ~ XMSS_MT_PRF.sign :
+      Glob.mem{1} = mem /\
+      Glob.mem{2} = mem /\
+
+      arg{1}.`1 = DecodeSkNoOID _sk /\
+      arg{1}.`2 = _sm_ptr /\
+      arg{1}.`3 = _smlen_ptr /\
+      arg{1}.`4 = _m_ptr /\
+      arg{1}.`5 = _mlen  /\
+
+      arg{2}.`1 =_sk /\
+      arg{2}.`2 = load_message mem _m_ptr _mlen /\
+
+      valid_ptr_i arg{1}.`5 2500 /\
+      2^XMSS_FULL_HEIGHT - 1 <= to_uint sk{2}.`idx (* the maximum number of signatures was reached *)
+      ==>
+      res{1}.`2 <> W64.zero
+    ].
+proof.
+rewrite /XMSS_N => [#] n_val ??.
+proc => /=.
+
+seq 11 5 : (
+  #pre /\
+  idx{2} = sk{2}.`Types.idx /\
+  2^XMSS_FULL_HEIGHT - 1 <= to_uint idx{1} /\
+  idx{2} = W32ofBytes (sub sk{1} 0 4) /\
+  exit_0{1} = W8.zero
+).
+    + admit.
+seq 7 0 : (#pre /\ to_uint idx{1} = to_uint idx{2}).
+    + admit.
+rcondt {1} 1.
+    + auto => /> &hr ?? H0 H1 ? H2. 
+      rewrite uleE of_uintK /(`<<`) // ifT //=.
+
+admit.
+qed.
+
+
+
+lemma sign_correct (mem : global_mem_t) (_sk : xmss_sk, _sm_ptr _smlen_ptr _m_ptr _mlen : W64.t) :
+    n = XMSS_N /\ 
+    prf_padding_val = XMSS_HASH_PADDING_PRF /\ 
+    padding_len = XMSS_PADDING_LEN =>
+    equiv [
+      M(Syscall).__xmssmt_core_sign ~ XMSS_MT_PRF.sign :
+      Glob.mem{1} = mem /\
+      Glob.mem{2} = mem /\
+
+      arg{1}.`1 = DecodeSkNoOID _sk /\
+      arg{1}.`2 = _sm_ptr /\
+      arg{1}.`3 = _smlen_ptr /\
+      arg{1}.`4 = _m_ptr /\
+      arg{1}.`5 = _mlen  /\
+
+      arg{2}.`1 =_sk /\
+      arg{2}.`2 = load_message mem _m_ptr _mlen /\
+
       valid_ptr_i arg{1}.`5 2500 /\
       0 <= to_uint sk{2}.`idx < 2^XMSS_FULL_HEIGHT - 1 (* ensures that the maximum number of signatures was not yet reached *)
       ==>
-      true
+(*      res{2}.`2 = DecodeSkNoOID res{2}.`1 *)
+      false
     ].
 proof.
-proc.
-
-swap {2} 5 -4.
-
-seq 12 1 : (
+rewrite /XMSS_N => [#] n_val ??.
+proc => /=.
+seq 13 5 : (
   #pre /\
   exit_0{1} = W8.zero /\
   ots_addr{1} = zero_addr /\
-  address{2} = ots_addr{1}
-); first by inline {1} M(Syscall).__zero_address_; wp; sp; ecall {1} (zero_addr_res addr{1}); skip => />. 
+  
+  idx{2} = sk{2}.`Types.idx /\
+  idx{2} = W32ofBytes (sub sk{1} 0 4) /\
 
-seq 2 0 : (#pre); first by admit. 
+  address{2} = zero_addr /\
+  root{2} = sk{2}.`sk_root /\
+  sk_prf{2} = sk{2}.`Types.sk_prf /\
 
-seq 2 0 : (#pre /\ to_uint t64{1} = to_uint mlen{1} + 2500). (* 2500 = XMSS_SIG_BYTES *) 
-    + auto => /> &1 *; rewrite to_uintD of_uintK /#. 
+  idx_new{2} = idx{2} + W32.one
+). 
 
-rcondf {1} 3.
-    + admit. 
+    + inline {1} 13.
+      inline {1} 12.
+      wp.
+      ecall {1} (zero_addr_res addr{1}).
+      auto => /> *.
+      split. 
+         * rewrite /zero_addr tP => i?.
+           rewrite get_setE // initiE //.
+         * admit.
+seq 1 0 : (#pre); first by admit.
+seq 2 0 : (#pre /\ to_uint t64{1} = to_uint mlen{1} + XMSS_SIG_BYTES). (* 2500 = XMSS_SIG_BYTES *) 
+    + auto => /> *; rewrite to_uintD of_uintK /#. 
+seq 1 0 : #pre; first by admit. (* memories are no longer equal *)
+seq 1 0 : (
+  #pre /\ 
+  to_uint idx{1} = to_uint (W32ofBytes (sub sk{1} 0 4)) /\
+  to_uint idx{1} = to_uint sk{2}.`Types.idx
+).
+    + admit. (* Add lemma to Correctness Bytes *)
+rcondf {1} 1.
+    + auto => /> &hr ???H H0 ?? H1. 
+      rewrite uleE of_uintK H1.  
+      rewrite /XMSS_FULL_HEIGHT /= in H.
+      rewrite /(`<<`) ifT // /= /#. 
+rcondt {1} 1; first by auto => /> *; smt(@W8).
+seq 1 0 : (#pre); first by admit. (* fix this *)
+seq 4 0 : (#pre /\ sub sk{1} 0 4 = lenbytes_be32 idx_new{2} 4); first by admit.
 
+swap {2} 2 - 1.
+seq 1 1 : (
+    #pre /\
+    to_list idx_bytes{1} = val idx_bytes{2}
+); first by admit. (* este idx e o original ou o que foi incrementado? ++> O original *)
+
+seq 0 1 : (#pre /\ sk{1} = DecodeSkNoOID sk{2}). (* Isto nao e #pre *)
+    + auto => /> &1 *; do split => />. 
+        * admit.
+        * rewrite to_uintD /#.
+        * move => ?. rewrite /XMSS_FULL_HEIGHT /= to_uintD. admit.
+        * admit.
+        * admit.
+        * admit.
+
+seq 1 0 : (#pre /\ to_list sk_prf{1} = val sk_prf{2}).
+    + auto => /> &1 &2 *.
+      apply (eq_from_nth witness); first by rewrite valP n_val size_to_list.
+      rewrite size_to_list => j?. 
+      rewrite get_to_list initiE // => />.
+      rewrite /DecodeSkNoOID get_of_list 1:/#.
+      rewrite nth_cat !size_cat !valP n_val sizeW32toBytes /= ifT 1:/#.
+      rewrite nth_cat !size_cat !valP n_val sizeW32toBytes /= ifT 1:/#.
+      by rewrite nth_cat !size_cat !valP n_val sizeW32toBytes /= ifF 1:/#.
+
+seq 1 1 : (#pre /\ to_list buf{1} = val _R{2}).
+    + inline {1} M(Syscall).__prf_ M(Syscall)._prf; wp; sp.
+      exists * in_00{1}, key0{1}; elim * => _P1 _P2; call {1} (prf_correctness _P1 _P2) => [/# |]. 
+      skip => /> &1 &2  ???? H0 H1 H2 H3 H4 H5 H6; do split. 
+        * rewrite H5 #smt:(@NBytes).
+        * rewrite H6 #smt:(@NBytes).
+        * by move => ???? ->.
+admit.
 qed.
